iris/ProofUsertrap.v
@@ -1250,9 +1250,10 @@ Lemma usertrap_res_bare_fd_tf_open
   ∃ kroot : mword 44,
     kpt_inv kroot ∗ ⌜tf_kernel_words_ok kroot ksp (pv_tf (us_V U))⌝ ∗
     tf_page (ud_tfp pt) (pv_tf (us_V U)) ∗
+    own_context cur_ctx ∗
     (∀ (ws' : list (mword 64)) (sts' : list fdstate),
        ⌜tf_kernel_words_ok kroot ksp ws'⌝ -∗ tf_page (ud_tfp pt) ws' -∗
-       FdSlots.fd_frags (pv_fdg (us_V U)) sts' -∗
+       FdSlots.fd_frags (pv_fdg (us_V U)) sts' -∗ own_context cur_ctx -∗
        usertrap_res_bare pt ksp (us_tf U ws') sts').
 Proof. exact (ut_res_bare_fd_tf_open SY.syscall_env pt ksp U sts). Qed.
 
@@ -1260,8 +1261,10 @@ Lemma usertrap_res_bare_fd_open
     `{!riscvGS Σ, !xv6G Σ, !bioslotG Σ, !fdslotG Σ, !fileG Σ, !irefslotG Σ, !pavG Σ} `{!ufdG Σ} `{GEN : GenId} `{CID : CpuId} `{XI : CurCtx} (pt : uptd) (ksp : mword 64) (U : ustate) (sts : list fdstate) :
   usertrap_res_bare pt ksp U sts -∗
   FdSlots.fd_frags (pv_fdg (us_V U)) sts ∗
+  own_context cur_ctx ∗
   (∀ sts' : list fdstate,
-     FdSlots.fd_frags (pv_fdg (us_V U)) sts' -∗ usertrap_res_bare pt ksp U sts').
+     FdSlots.fd_frags (pv_fdg (us_V U)) sts' -∗ own_context cur_ctx -∗
+     usertrap_res_bare pt ksp U sts').
 Proof. exact (ut_res_bare_fd_open SY.syscall_env pt ksp U sts). Qed.
 
 Lemma usertrap_res_bare_norm
@@ -1276,8 +1279,10 @@ Lemma usertrap_res_tf_open
   ∃ kroot : mword 44,
     kpt_inv kroot ∗ ⌜tf_kernel_words_ok kroot ksp (pv_tf (us_V U))⌝ ∗
     tf_page (ud_tfp pt) (pv_tf (us_V U)) ∗
+    own_context cur_ctx ∗
     (∀ ws' : list (mword 64),
        ⌜tf_kernel_words_ok kroot ksp ws'⌝ -∗ tf_page (ud_tfp pt) ws' -∗
+     own_context cur_ctx -∗
        usertrap_res_bare pt ksp (us_tf U ws') sts).
 Proof. exact (ut_res_bare_tf_open SY.syscall_env pt ksp U sts). Qed.
 
@@ -1313,9 +1318,9 @@ Lemma usertrap_res_tf_csrs_open
   usertrap_res_bare pt ksp U sts -∗
   ∃ kroot : mword 44,
     kpt_inv kroot ∗ ⌜tf_kernel_words_ok kroot ksp (pv_tf (us_V U))⌝ ∗
-    tf_page (ud_tfp pt) (pv_tf (us_V U)) ∗ hart_csrs ∗
+    tf_page (ud_tfp pt) (pv_tf (us_V U)) ∗ hart_csrs ∗ own_context cur_ctx ∗
     (∀ ws' : list (mword 64),
-       ⌜tf_kernel_words_ok kroot ksp ws'⌝ -∗ tf_page (ud_tfp pt) ws' -∗ hart_csrs -∗
+       ⌜tf_kernel_words_ok kroot ksp ws'⌝ -∗ tf_page (ud_tfp pt) ws' -∗ hart_csrs -∗ own_context cur_ctx -∗
        usertrap_res_bare pt ksp (us_tf U ws') sts).
 Proof. exact (ut_res_bare_tf_csrs_open SY.syscall_env pt ksp U sts). Qed.
 
